backend/Cmconstrproof.v
@@ -67,38 +67,38 @@ Scheme eval_expr_ind_3 := Minimality for eval_expr Sort Prop
   with eval_condexpr_ind_3 := Minimality for eval_condexpr Sort Prop
   with eval_exprlist_ind_3 := Minimality for eval_exprlist Sort Prop.
 
-Hint Resolve eval_Evar eval_Eassign eval_Eop eval_Eload eval_Estore
+Hint Resolve eval_Evar eval_Eop eval_Eload eval_Estore
              eval_Ecall eval_Econdition eval_Ealloc
              eval_Elet eval_Eletvar 
              eval_CEtrue eval_CEfalse eval_CEcond
              eval_CEcondition eval_Enil eval_Econs: evalexpr.
 
 Lemma eval_list_one:
-  forall sp le e1 m1 a t e2 m2 v,
-  eval_expr ge sp le e1 m1 a t e2 m2 v ->
-  eval_exprlist ge sp le e1 m1 (a ::: Enil) t e2 m2 (v :: nil).
+  forall sp le e m1 a t m2 v,
+  eval_expr ge sp le e m1 a t m2 v ->
+  eval_exprlist ge sp le e m1 (a ::: Enil) t m2 (v :: nil).
 Proof.
   intros. econstructor. eauto. constructor. traceEq.
 Qed.
 
 Lemma eval_list_two:
-  forall sp le e1 m1 a1 t1 e2 m2 v1 a2 t2 e3 m3 v2 t,
-  eval_expr ge sp le e1 m1 a1 t1 e2 m2 v1 ->
-  eval_expr ge sp le e2 m2 a2 t2 e3 m3 v2 ->
+  forall sp le e m1 a1 t1 m2 v1 a2 t2 m3 v2 t,
+  eval_expr ge sp le e m1 a1 t1 m2 v1 ->
+  eval_expr ge sp le e m2 a2 t2 m3 v2 ->
   t = t1 ** t2 ->
-  eval_exprlist ge sp le e1 m1 (a1 ::: a2 ::: Enil) t e3 m3 (v1 :: v2 :: nil).
+  eval_exprlist ge sp le e m1 (a1 ::: a2 ::: Enil) t m3 (v1 :: v2 :: nil).
 Proof.
   intros. econstructor. eauto. econstructor. eauto. constructor. 
   reflexivity. traceEq.
 Qed.
 
 Lemma eval_list_three:
-  forall sp le e1 m1 a1 t1 e2 m2 v1 a2 t2 e3 m3 v2 a3 t3 e4 m4 v3 t,
-  eval_expr ge sp le e1 m1 a1 t1 e2 m2 v1 ->
-  eval_expr ge sp le e2 m2 a2 t2 e3 m3 v2 ->
-  eval_expr ge sp le e3 m3 a3 t3 e4 m4 v3 ->
+  forall sp le e m1 a1 t1 m2 v1 a2 t2 m3 v2 a3 t3 m4 v3 t,
+  eval_expr ge sp le e m1 a1 t1 m2 v1 ->
+  eval_expr ge sp le e m2 a2 t2 m3 v2 ->
+  eval_expr ge sp le e m3 a3 t3 m4 v3 ->
   t = t1 ** t2 ** t3 ->
-  eval_exprlist ge sp le e1 m1 (a1 ::: a2 ::: a3 ::: Enil) t e4 m4 (v1 :: v2 :: v3 :: nil).
+  eval_exprlist ge sp le e m1 (a1 ::: a2 ::: a3 ::: Enil) t m4 (v1 :: v2 :: v3 :: nil).
 Proof.
   intros. econstructor. eauto. econstructor. eauto. econstructor. eauto. constructor. 
   reflexivity. reflexivity. traceEq.
@@ -107,22 +107,22 @@ Qed.
 Hint Resolve eval_list_one eval_list_two eval_list_three: evalexpr.
 
 Lemma eval_lift_expr:
-  forall w sp le e1 m1 a t e2 m2 v,
-  eval_expr ge sp le e1 m1 a t e2 m2 v ->
+  forall w sp le e m1 a t m2 v,
+  eval_expr ge sp le e m1 a t m2 v ->
   forall p le', insert_lenv le p w le' ->
-  eval_expr ge sp le' e1 m1 (lift_expr p a) t e2 m2 v.
+  eval_expr ge sp le' e m1 (lift_expr p a) t m2 v.
 Proof.
   intros w.
   apply (eval_expr_ind_3 ge
-    (fun sp le e1 m1 a t e2 m2 v =>
+    (fun sp le e m1 a t m2 v =>
       forall p le', insert_lenv le p w le' ->
-      eval_expr ge sp le' e1 m1 (lift_expr p a) t e2 m2 v)
-    (fun sp le e1 m1 a t e2 m2 vb =>
+      eval_expr ge sp le' e m1 (lift_expr p a) t m2 v)
+    (fun sp le e m1 a t m2 vb =>
       forall p le', insert_lenv le p w le' ->
-      eval_condexpr ge sp le' e1 m1 (lift_condexpr p a) t e2 m2 vb)
-    (fun sp le e1 m1 al t e2 m2 vl =>
+      eval_condexpr ge sp le' e m1 (lift_condexpr p a) t m2 vb)
+    (fun sp le e m1 al t m2 vl =>
       forall p le', insert_lenv le p w le' ->
-      eval_exprlist ge sp le' e1 m1 (lift_exprlist p al) t e2 m2 vl));
+      eval_exprlist ge sp le' e m1 (lift_exprlist p al) t m2 vl));
   simpl; intros; eauto with evalexpr.
 
   destruct v1; eapply eval_Econdition;
@@ -139,9 +139,9 @@ Proof.
 Qed.
 
 Lemma eval_lift:
-  forall sp le e1 m1 a t e2 m2 v w,
-  eval_expr ge sp le e1 m1 a t e2 m2 v ->
-  eval_expr ge sp (w::le) e1 m1 (lift a) t e2 m2 v.
+  forall sp le e m1 a t m2 v w,
+  eval_expr ge sp le e m1 a t m2 v ->
+  eval_expr ge sp (w::le) e m1 (lift a) t m2 v.
 Proof.
   intros. unfold lift. eapply eval_lift_expr.
   eexact H. apply insert_lenv_0. 
@@ -160,69 +160,69 @@ Ltac TrivialOp cstr :=
   of operator applications. *)  
 
 Lemma inv_eval_Eop_0:
-  forall sp le e1 m1 op t e2 m2 v,
-  eval_expr ge sp le e1 m1 (Eop op Enil) t e2 m2 v ->
-  t = E0 /\ e2 = e1 /\ m2 = m1 /\ eval_operation ge sp op nil = Some v.
+  forall sp le e m1 op t m2 v,
+  eval_expr ge sp le e m1 (Eop op Enil) t m2 v ->
+  t = E0 /\ m2 = m1 /\ eval_operation ge sp op nil = Some v.
 Proof.
   intros. inversion H. inversion H6. 
   intuition. congruence.
 Qed.
   
 Lemma inv_eval_Eop_1:
-  forall sp le e1 m1 op t a1 e2 m2 v,
-  eval_expr ge sp le e1 m1 (Eop op (a1 ::: Enil)) t e2 m2 v ->
+  forall sp le e m1 op t a1 m2 v,
+  eval_expr ge sp le e m1 (Eop op (a1 ::: Enil)) t m2 v ->
   exists v1,
-  eval_expr ge sp le e1 m1 a1 t e2 m2 v1 /\
+  eval_expr ge sp le e m1 a1 t m2 v1 /\
   eval_operation ge sp op (v1 :: nil) = Some v.
 Proof.
   intros. 
-  inversion H. inversion H6. inversion H19. 
+  inversion H. inversion H6. inversion H18. 
   subst. exists v1; intuition. rewrite E0_right. auto.
 Qed.
 
 Lemma inv_eval_Eop_2:
-  forall sp le e1 m1 op a1 a2 t3 e3 m3 v,
-  eval_expr ge sp le e1 m1 (Eop op (a1 ::: a2 ::: Enil)) t3 e3 m3 v ->
-  exists t1, exists t2, exists e2, exists m2, exists v1, exists v2,
-  eval_expr ge sp le e1 m1 a1 t1 e2 m2 v1 /\
-  eval_expr ge sp le e2 m2 a2 t2 e3 m3 v2 /\
+  forall sp le e m1 op a1 a2 t3 m3 v,
+  eval_expr ge sp le e m1 (Eop op (a1 ::: a2 ::: Enil)) t3 m3 v ->
+  exists t1, exists t2, exists m2, exists v1, exists v2,
+  eval_expr ge sp le e m1 a1 t1 m2 v1 /\
+  eval_expr ge sp le e m2 a2 t2 m3 v2 /\
   t3 = t1 ** t2 /\
   eval_operation ge sp op (v1 :: v2 :: nil) = Some v.
 Proof.
   intros. 
   inversion H. subst. inversion H6. subst. inversion H8. subst.
-  inversion H10. subst. 
-  exists t1; exists t0; exists e0; exists m0; exists v0; exists v1.
+  inversion H11. subst. 
+  exists t1; exists t0; exists m0; exists v0; exists v1.
   intuition. traceEq.
 Qed.
 
 Ltac SimplEval :=
   match goal with
-  | [ |- (eval_expr _ ?sp ?le ?e1 ?m1 (Eop ?op Enil) ?t ?e2 ?m2 ?v) -> _] =>
+  | [ |- (eval_expr _ ?sp ?le ?e ?m1 (Eop ?op Enil) ?t ?m2 ?v) -> _] =>
       intro XX1;
-      generalize (inv_eval_Eop_0 sp le e1 m1 op t e2 m2 v XX1);
+      generalize (inv_eval_Eop_0 sp le e m1 op t m2 v XX1);
       clear XX1;
-      intros [XX1 [XX2 [XX3 XX4]]];
-      subst t e2 m2; simpl in XX4; 
-      try (simplify_eq XX4; clear XX4;
+      intros [XX1 [XX2 XX3]];
+      subst t m2; simpl in XX3; 
+      try (simplify_eq XX3; clear XX3;
       let EQ := fresh "EQ" in (intro EQ; rewrite EQ))
-  | [ |- (eval_expr _ ?sp ?le ?e1 ?m1 (Eop ?op (?a1 ::: Enil)) ?t ?e2 ?m2 ?v) -> _] =>
+  | [ |- (eval_expr _ ?sp ?le ?e ?m1 (Eop ?op (?a1 ::: Enil)) ?t ?m2 ?v) -> _] =>
       intro XX1;
-      generalize (inv_eval_Eop_1 sp le e1 m1 op t a1 e2 m2 v XX1);
+      generalize (inv_eval_Eop_1 sp le e m1 op t a1 m2 v XX1);
       clear XX1;
       let v1 := fresh "v" in let EV := fresh "EV" in
       let EQ := fresh "EQ" in
       (intros [v1 [EV EQ]]; simpl in EQ)
-  | [ |- (eval_expr _ ?sp ?le ?e1 ?m1 (Eop ?op (?a1 ::: ?a2 ::: Enil)) ?t ?e2 ?m2 ?v) -> _] =>
+  | [ |- (eval_expr _ ?sp ?le ?e ?m1 (Eop ?op (?a1 ::: ?a2 ::: Enil)) ?t ?m2 ?v) -> _] =>
       intro XX1;
-      generalize (inv_eval_Eop_2 sp le e1 m1 op a1 a2 t e2 m2 v XX1);
+      generalize (inv_eval_Eop_2 sp le e m1 op a1 a2 t m2 v XX1);
       clear XX1;
       let t1 := fresh "t" in let t2 := fresh "t" in
-      let e := fresh "e" in let m := fresh "m" in
+      let m := fresh "m" in
       let v1 := fresh "v" in let v2 := fresh "v" in
       let EV1 := fresh "EV" in let EV2 := fresh "EV" in
       let EQ := fresh "EQ" in let TR := fresh "TR" in
-      (intros [t1 [t2 [e [m [v1 [v2 [EV1 [EV2 [TR EQ]]]]]]]]]; simpl in EQ)
+      (intros [t1 [t2 [m [v1 [v2 [EV1 [EV2 [TR EQ]]]]]]]]; simpl in EQ)
   | _ => idtac
   end.
 
@@ -245,57 +245,57 @@ Ltac InvEval H :=
 *)
 
 Theorem eval_negint:
-  forall sp le e1 m1 a t e2 m2 x,
-  eval_expr ge sp le e1 m1 a t e2 m2 (Vint x) ->
-  eval_expr ge sp le e1 m1 (negint a) t e2 m2 (Vint (Int.neg x)).
+  forall sp le e m1 a t m2 x,
+  eval_expr ge sp le e m1 a t m2 (Vint x) ->
+  eval_expr ge sp le e m1 (negint a) t m2 (Vint (Int.neg x)).
 Proof.
   TrivialOp negint. 
 Qed.
 
 Theorem eval_negfloat:
-  forall sp le e1 m1 a t e2 m2 x,
-  eval_expr ge sp le e1 m1 a t e2 m2 (Vfloat x) ->
-  eval_expr ge sp le e1 m1 (negfloat a) t e2 m2 (Vfloat (Float.neg x)).
+  forall sp le e m1 a t m2 x,
+  eval_expr ge sp le e m1 a t m2 (Vfloat x) ->
+  eval_expr ge sp le e m1 (negfloat a) t m2 (Vfloat (Float.neg x)).
 Proof.
   TrivialOp negfloat.
 Qed.
 
 Theorem eval_absfloat:
-  forall sp le e1 m1 a t e2 m2 x,
-  eval_expr ge sp le e1 m1 a t e2 m2 (Vfloat x) ->
-  eval_expr ge sp le e1 m1 (absfloat a) t e2 m2 (Vfloat (Float.abs x)).
+  forall sp le e m1 a t m2 x,
+  eval_expr ge sp le e m1 a t m2 (Vfloat x) ->
+  eval_expr ge sp le e m1 (absfloat a) t m2 (Vfloat (Float.abs x)).
 Proof.
   TrivialOp absfloat.
 Qed.
 
 Theorem eval_intoffloat:
-  forall sp le e1 m1 a t e2 m2 x,
-  eval_expr ge sp le e1 m1 a t e2 m2 (Vfloat x) ->
-  eval_expr ge sp le e1 m1 (intoffloat a) t e2 m2 (Vint (Float.intoffloat x)).
+  forall sp le e m1 a t m2 x,
+  eval_expr ge sp le e m1 a t m2 (Vfloat x) ->
+  eval_expr ge sp le e m1 (intoffloat a) t m2 (Vint (Float.intoffloat x)).
 Proof.
   TrivialOp intoffloat.
 Qed.
 
 Theorem eval_floatofint:
-  forall sp le e1 m1 a t e2 m2 x,
-  eval_expr ge sp le e1 m1 a t e2 m2 (Vint x) ->
-  eval_expr ge sp le e1 m1 (floatofint a) t e2 m2 (Vfloat (Float.floatofint x)).
+  forall sp le e m1 a t m2 x,
+  eval_expr ge sp le e m1 a t m2 (Vint x) ->
+  eval_expr ge sp le e m1 (floatofint a) t m2 (Vfloat (Float.floatofint x)).
 Proof.
   TrivialOp floatofint.
 Qed.
 
 Theorem eval_floatofintu:
-  forall sp le e1 m1 a t e2 m2 x,
-  eval_expr ge sp le e1 m1 a t e2 m2 (Vint x) ->
-  eval_expr ge sp le e1 m1 (floatofintu a) t e2 m2 (Vfloat (Float.floatofintu x)).
+  forall sp le e m1 a t m2 x,
+  eval_expr ge sp le e m1 a t m2 (Vint x) ->
+  eval_expr ge sp le e m1 (floatofintu a) t m2 (Vfloat (Float.floatofintu x)).
 Proof.
   TrivialOp floatofintu.
 Qed.
 
 Theorem eval_notint:
-  forall sp le e1 m1 a t e2 m2 x,
-  eval_expr ge sp le e1 m1 a t e2 m2 (Vint x) ->
-  eval_expr ge sp le e1 m1 (notint a) t e2 m2 (Vint (Int.not x)).
+  forall sp le e m1 a t m2 x,
+  eval_expr ge sp le e m1 a t m2 (Vint x) ->
+  eval_expr ge sp le e m1 (notint a) t m2 (Vint (Int.not x)).
 Proof.
   unfold notint; intros until x; case (notint_match a); intros.
   InvEval H. FuncInv. EvalOp. simpl. congruence. 
@@ -310,10 +310,10 @@ Proof.
 Qed.
 
 Lemma eval_notbool_base:
-  forall sp le e1 m1 a t e2 m2 v b,
-  eval_expr ge sp le e1 m1 a t e2 m2 v ->
+  forall sp le e m1 a t m2 v b,
+  eval_expr ge sp le e m1 a t m2 v ->
   Val.bool_of_val v b ->
-  eval_expr ge sp le e1 m1 (notbool_base a) t e2 m2 (Val.of_bool (negb b)).
+  eval_expr ge sp le e m1 (notbool_base a) t m2 (Val.of_bool (negb b)).
 Proof. 
   TrivialOp notbool_base. simpl. 
   inversion H0. 
@@ -326,10 +326,10 @@ Hint Resolve Val.bool_of_true_val Val.bool_of_false_val
              Val.bool_of_true_val_inv Val.bool_of_false_val_inv: valboolof.
 
 Theorem eval_notbool:
-  forall a sp le e1 m1 t e2 m2 v b,
-  eval_expr ge sp le e1 m1 a t e2 m2 v ->
+  forall a sp le e m1 t m2 v b,
+  eval_expr ge sp le e m1 a t m2 v ->
   Val.bool_of_val v b ->
-  eval_expr ge sp le e1 m1 (notbool a) t e2 m2 (Val.of_bool (negb b)).
+  eval_expr ge sp le e m1 (notbool a) t m2 (Val.of_bool (negb b)).
 Proof.
   assert (N1: forall v b, Val.is_false v -> Val.bool_of_val v b -> Val.is_true (Val.of_bool (negb b))).
     intros. inversion H0; simpl; auto; subst v; simpl in H.
@@ -341,33 +341,33 @@ Proof.
   induction a; simpl; intros; try (eapply eval_notbool_base; eauto).
   destruct o; try (eapply eval_notbool_base; eauto).
 
-  destruct e. InvEval H. injection XX4; clear XX4; intro; subst v.
+  destruct e. InvEval H. injection XX3; clear XX3; intro; subst v.
   inversion H0. rewrite Int.eq_false; auto. 
   simpl; eauto with evalexpr.
   rewrite Int.eq_true; simpl; eauto with evalexpr.
   eapply eval_notbool_base; eauto.
 
   inversion H. subst. 
-  simpl in H12. eapply eval_Eop; eauto.
+  simpl in H11. eapply eval_Eop; eauto.
   simpl. caseEq (eval_condition c vl); intros.
-  rewrite H1 in H12. 
+  rewrite H1 in H11. 
   assert (b0 = b). 
-  destruct b0; inversion H12; subst v; inversion H0; auto.
+  destruct b0; inversion H11; subst v; inversion H0; auto.
   subst b0. rewrite (Op.eval_negate_condition _ _ H1). 
   destruct b; reflexivity.
-  rewrite H1 in H12; discriminate.
+  rewrite H1 in H11; discriminate.
 
   inversion H; eauto 10 with evalexpr valboolof.
   inversion H; eauto 10 with evalexpr valboolof.
 
-  inversion H. subst. eapply eval_Econdition with (t2 := t8). eexact H36.
+  inversion H. subst. eapply eval_Econdition with (t2 := t8). eexact H34.
   destruct v4; eauto. auto.
 Qed.
 
 Theorem eval_addimm:
-  forall sp le e1 m1 n a t e2 m2 x,
-  eval_expr ge sp le e1 m1 a t e2 m2 (Vint x) ->
-  eval_expr ge sp le e1 m1 (addimm n a) t e2 m2 (Vint (Int.add x n)).
+  forall sp le e m1 n a t m2 x,
+  eval_expr ge sp le e m1 a t m2 (Vint x) ->
+  eval_expr ge sp le e m1 (addimm n a) t m2 (Vint (Int.add x n)).
 Proof.
   unfold addimm; intros until x.
   generalize (Int.eq_spec n Int.zero). case (Int.eq n Int.zero); intro.
@@ -376,16 +376,16 @@ Proof.
   InvEval H0. EvalOp. simpl. rewrite Int.add_commut. auto.
   InvEval H0. destruct (Genv.find_symbol ge s); discriminate.
   InvEval H0. 
-  destruct sp; simpl in XX4; discriminate.
+  destruct sp; simpl in XX3; discriminate.
   InvEval H0. FuncInv. EvalOp. simpl. subst x. 
   rewrite Int.add_assoc. decEq; decEq; decEq. apply Int.add_commut.
   EvalOp. 
 Qed. 
 
 Theorem eval_addimm_ptr:
-  forall sp le e1 m1 n t a e2 m2 b ofs,
-  eval_expr ge sp le e1 m1 a t e2 m2 (Vptr b ofs) ->
-  eval_expr ge sp le e1 m1 (addimm n a) t e2 m2 (Vptr b (Int.add ofs n)).
+  forall sp le e m1 n t a m2 b ofs,
+  eval_expr ge sp le e m1 a t m2 (Vptr b ofs) ->
+  eval_expr ge sp le e m1 (addimm n a) t m2 (Vptr b (Int.add ofs n)).
 Proof.
   unfold addimm; intros until ofs.
   generalize (Int.eq_spec n Int.zero). case (Int.eq n Int.zero); intro.
@@ -396,8 +396,8 @@ Proof.
     destruct (Genv.find_symbol ge s). 
     rewrite Int.add_commut. congruence.
     discriminate.
-  InvEval H0. destruct sp; simpl in XX4; try discriminate.
-  inversion XX4. EvalOp. simpl. decEq. decEq. 
+  InvEval H0. destruct sp; simpl in XX3; try discriminate.
+  inversion XX3. EvalOp. simpl. decEq. decEq. 
   rewrite Int.add_assoc. decEq. apply Int.add_commut.
   InvEval H0. FuncInv. subst b0; subst ofs. EvalOp. simpl. 
     rewrite (Int.add_commut n m). rewrite Int.add_assoc. auto.
@@ -405,10 +405,10 @@ Proof.
 Qed.
 
 Theorem eval_add:
-  forall sp le e1 m1 a t1 e2 m2 x b t2 e3 m3 y,
-  eval_expr ge sp le e1 m1 a t1 e2 m2 (Vint x) ->
-  eval_expr ge sp le e2 m2 b t2 e3 m3 (Vint y) ->
-  eval_expr ge sp le e1 m1 (add a b) (t1**t2) e3 m3 (Vint (Int.add x y)).
+  forall sp le e m1 a t1 m2 x b t2 m3 y,
+  eval_expr ge sp le e m1 a t1 m2 (Vint x) ->
+  eval_expr ge sp le e m2 b t2 m3 (Vint y) ->
+  eval_expr ge sp le e m1 (add a b) (t1**t2) m3 (Vint (Int.add x y)).
 Proof.
   intros until y. unfold add; case (add_match a b); intros.
   InvEval H. rewrite Int.add_commut. apply eval_addimm. 
@@ -432,10 +432,10 @@ Proof.
 Qed.
 
 Theorem eval_add_ptr:
-  forall sp le e1 m1 a t1 e2 m2 p x b t2 e3 m3 y,
-  eval_expr ge sp le e1 m1 a t1 e2 m2 (Vptr p x) ->
-  eval_expr ge sp le e2 m2 b t2 e3 m3 (Vint y) ->
-  eval_expr ge sp le e1 m1 (add a b) (t1**t2) e3 m3 (Vptr p (Int.add x y)).
+  forall sp le e m1 a t1 m2 p x b t2 m3 y,
+  eval_expr ge sp le e m1 a t1 m2 (Vptr p x) ->
+  eval_expr ge sp le e m2 b t2 m3 (Vint y) ->
+  eval_expr ge sp le e m1 (add a b) (t1**t2) m3 (Vptr p (Int.add x y)).
 Proof.
   intros until y. unfold add; case (add_match a b); intros.
   InvEval H. 
@@ -457,10 +457,10 @@ Proof.
 Qed.
 
 Theorem eval_add_ptr_2:
-  forall sp le e1 m1 a t1 e2 m2 p x b t2 e3 m3 y,
-  eval_expr ge sp le e1 m1 a t1 e2 m2 (Vint x) ->
-  eval_expr ge sp le e2 m2 b t2 e3 m3 (Vptr p y) ->
-  eval_expr ge sp le e1 m1 (add a b) (t1**t2) e3 m3 (Vptr p (Int.add y x)).
+  forall sp le e m1 a t1 m2 p x b t2 m3 y,
+  eval_expr ge sp le e m1 a t1 m2 (Vint x) ->
+  eval_expr ge sp le e m2 b t2 m3 (Vptr p y) ->
+  eval_expr ge sp le e m1 (add a b) (t1**t2) m3 (Vptr p (Int.add y x)).
 Proof.
   intros until y. unfold add; case (add_match a b); intros.
   InvEval H. 
@@ -484,10 +484,10 @@ Proof.
 Qed.
 
 Theorem eval_sub:
-  forall sp le e1 m1 a t1 e2 m2 x b t2 e3 m3 y,
-  eval_expr ge sp le e1 m1 a t1 e2 m2 (Vint x) ->
-  eval_expr ge sp le e2 m2 b t2 e3 m3 (Vint y) ->
-  eval_expr ge sp le e1 m1 (sub a b) (t1**t2) e3 m3 (Vint (Int.sub x y)).
+  forall sp le e m1 a t1 m2 x b t2 m3 y,
+  eval_expr ge sp le e m1 a t1 m2 (Vint x) ->
+  eval_expr ge sp le e m2 b t2 m3 (Vint y) ->
+  eval_expr ge sp le e m1 (sub a b) (t1**t2) m3 (Vint (Int.sub x y)).
 Proof.
   intros until y.
   unfold sub; case (sub_match a b); intros.
@@ -512,10 +512,10 @@ Proof.
 Qed.
 
 Theorem eval_sub_ptr_int:
-  forall sp le e1 m1 a t1 e2 m2 p x b t2 e3 m3 y,
-  eval_expr ge sp le e1 m1 a t1 e2 m2 (Vptr p x) ->
-  eval_expr ge sp le e2 m2 b t2 e3 m3 (Vint y) ->
-  eval_expr ge sp le e1 m1 (sub a b) (t1**t2) e3 m3 (Vptr p (Int.sub x y)).
+  forall sp le e m1 a t1 m2 p x b t2 m3 y,
+  eval_expr ge sp le e m1 a t1 m2 (Vptr p x) ->
+  eval_expr ge sp le e m2 b t2 m3 (Vint y) ->
+  eval_expr ge sp le e m1 (sub a b) (t1**t2) m3 (Vptr p (Int.sub x y)).
 Proof.
   intros until y.
   unfold sub; case (sub_match a b); intros.
@@ -541,10 +541,10 @@ Proof.
 Qed.
 
 Theorem eval_sub_ptr_ptr:
-  forall sp le e1 m1 a t1 e2 m2 p x b t2 e3 m3 y,
-  eval_expr ge sp le e1 m1 a t1 e2 m2 (Vptr p x) ->
-  eval_expr ge sp le e2 m2 b t2 e3 m3 (Vptr p y) ->
-  eval_expr ge sp le e1 m1 (sub a b) (t1**t2) e3 m3 (Vint (Int.sub x y)).
+  forall sp le e m1 a t1 m2 p x b t2 m3 y,
+  eval_expr ge sp le e m1 a t1 m2 (Vptr p x) ->
+  eval_expr ge sp le e m2 b t2 m3 (Vptr p y) ->
+  eval_expr ge sp le e m1 (sub a b) (t1**t2) m3 (Vint (Int.sub x y)).
 Proof.
   intros until y.
   unfold sub; case (sub_match a b); intros.
@@ -571,9 +571,9 @@ Proof.
 Qed.
 
 Lemma eval_rolm:
-  forall sp le e1 m1 a amount mask t e2 m2 x,
-  eval_expr ge sp le e1 m1 a t e2 m2 (Vint x) ->
-  eval_expr ge sp le e1 m1 (rolm a amount mask) t e2 m2 (Vint (Int.rolm x amount mask)).
+  forall sp le e m1 a amount mask t m2 x,
+  eval_expr ge sp le e m1 a t m2 (Vint x) ->
+  eval_expr ge sp le e m1 (rolm a amount mask) t m2 (Vint (Int.rolm x amount mask)).
 Proof.
   intros until x. unfold rolm; case (rolm_match a); intros.
   InvEval H. eauto with evalexpr. 
@@ -590,10 +590,10 @@ Proof.
 Qed.
 
 Theorem eval_shlimm:
-  forall sp le e1 m1 a n t e2 m2 x,
-  eval_expr ge sp le e1 m1 a t e2 m2 (Vint x) ->
+  forall sp le e m1 a n t m2 x,
+  eval_expr ge sp le e m1 a t m2 (Vint x) ->
   Int.ltu n (Int.repr 32) = true ->
-  eval_expr ge sp le e1 m1 (shlimm a n) t e2 m2 (Vint (Int.shl x n)).
+  eval_expr ge sp le e m1 (shlimm a n) t m2 (Vint (Int.shl x n)).
 Proof.
   intros.  unfold shlimm.
   generalize (Int.eq_spec n Int.zero); case (Int.eq n Int.zero); intro.
@@ -604,10 +604,10 @@ Proof.
 Qed.
 
 Theorem eval_shruimm:
-  forall sp le e1 m1 a n t e2 m2 x,
-  eval_expr ge sp le e1 m1 a t e2 m2 (Vint x) ->
+  forall sp le e m1 a n t m2 x,
+  eval_expr ge sp le e m1 a t m2 (Vint x) ->
   Int.ltu n (Int.repr 32) = true ->
-  eval_expr ge sp le e1 m1 (shruimm a n) t e2 m2 (Vint (Int.shru x n)).
+  eval_expr ge sp le e m1 (shruimm a n) t m2 (Vint (Int.shru x n)).
 Proof.
   intros.  unfold shruimm.
   generalize (Int.eq_spec n Int.zero); case (Int.eq n Int.zero); intro.
@@ -618,9 +618,9 @@ Proof.
 Qed.
 
 Lemma eval_mulimm_base:
-  forall sp le e1 m1 a t n e2 m2 x,
-  eval_expr ge sp le e1 m1 a t e2 m2 (Vint x) ->
-  eval_expr ge sp le e1 m1 (mulimm_base n a) t e2 m2 (Vint (Int.mul x n)).
+  forall sp le e m1 a t n m2 x,
+  eval_expr ge sp le e m1 a t m2 (Vint x) ->
+  eval_expr ge sp le e m1 (mulimm_base n a) t m2 (Vint (Int.mul x n)).
 Proof.
   intros; unfold mulimm_base. 
   generalize (Int.one_bits_decomp n). 
@@ -633,7 +633,7 @@ Proof.
   rewrite Int.add_zero. rewrite <- Int.shl_mul.
   apply eval_shlimm. auto. auto with coqlib. 
   destruct l.
-  intros. apply eval_Elet with t e2 m2 (Vint x) E0. auto.
+  intros. apply eval_Elet with t m2 (Vint x) E0. auto.
   rewrite H1. simpl. rewrite Int.add_zero. 
   rewrite Int.mul_add_distr_r.
   rewrite <- Int.shl_mul.
@@ -650,9 +650,9 @@ Proof.
 Qed.
 
 Theorem eval_mulimm:
-  forall sp le e1 m1 a n t e2 m2 x,
-  eval_expr ge sp le e1 m1 a t e2 m2 (Vint x) ->
-  eval_expr ge sp le e1 m1 (mulimm n a) t e2 m2 (Vint (Int.mul x n)).
+  forall sp le e m1 a n t m2 x,
+  eval_expr ge sp le e m1 a t m2 (Vint x) ->
+  eval_expr ge sp le e m1 (mulimm n a) t m2 (Vint (Int.mul x n)).
 Proof.
   intros until x; unfold mulimm.
   generalize (Int.eq_spec n Int.zero); case (Int.eq n Int.zero); intro.
@@ -670,10 +670,10 @@ Proof.
 Qed.
 
 Theorem eval_mul:
-  forall sp le e1 m1 a t1 e2 m2 x b t2 e3 m3 y,
-  eval_expr ge sp le e1 m1 a t1 e2 m2 (Vint x) ->
-  eval_expr ge sp le e2 m2 b t2 e3 m3 (Vint y) ->
-  eval_expr ge sp le e1 m1 (mul a b) (t1**t2) e3 m3 (Vint (Int.mul x y)).
+  forall sp le e m1 a t1 m2 x b t2 m3 y,
+  eval_expr ge sp le e m1 a t1 m2 (Vint x) ->
+  eval_expr ge sp le e m2 b t2 m3 (Vint y) ->
+  eval_expr ge sp le e m1 (mul a b) (t1**t2) m3 (Vint (Int.mul x y)).
 Proof.
   intros until y.
   unfold mul; case (mul_match a b); intros.
@@ -684,11 +684,11 @@ Proof.
 Qed.
 
 Theorem eval_divs:
-  forall sp le e1 m1 a t1 e2 m2 x b t2 e3 m3 y,
-  eval_expr ge sp le e1 m1 a t1 e2 m2 (Vint x) ->
-  eval_expr ge sp le e2 m2 b t2 e3 m3 (Vint y) ->
+  forall sp le e m1 a t1 m2 x b t2 m3 y,
+  eval_expr ge sp le e m1 a t1 m2 (Vint x) ->
+  eval_expr ge sp le e m2 b t2 m3 (Vint y) ->
   y <> Int.zero ->
-  eval_expr ge sp le e1 m1 (divs a b) (t1**t2) e3 m3 (Vint (Int.divs x y)).
+  eval_expr ge sp le e m1 (divs a b) (t1**t2) m3 (Vint (Int.divs x y)).
 Proof.
   TrivialOp divs. simpl. 
   predSpec Int.eq Int.eq_spec y Int.zero. contradiction. auto.
@@ -700,11 +700,11 @@ Lemma eval_mod_aux:
    y <> Int.zero ->
    eval_operation ge sp divop (Vint x :: Vint y :: nil) =
    Some (Vint (semdivop x y))) ->
-  forall sp le e1 m1 a t1 e2 m2 x b t2 e3 m3 y,
-  eval_expr ge sp le e1 m1 a t1 e2 m2 (Vint x) ->
-  eval_expr ge sp le e2 m2 b t2 e3 m3 (Vint y) ->
+  forall sp le e m1 a t1 m2 x b t2 m3 y,
+  eval_expr ge sp le e m1 a t1 m2 (Vint x) ->
+  eval_expr ge sp le e m2 b t2 m3 (Vint y) ->
   y <> Int.zero ->
-  eval_expr ge sp le e1 m1 (mod_aux divop a b) (t1**t2) e3 m3
+  eval_expr ge sp le e m1 (mod_aux divop a b) (t1**t2) m3
    (Vint (Int.sub x (Int.mul (semdivop x y) y))).
 Proof.
   intros; unfold mod_aux.
@@ -726,11 +726,11 @@ Proof.
 Qed.
 
 Theorem eval_mods:
-  forall sp le e1 m1 a t1 e2 m2 x b t2 e3 m3 y,
-  eval_expr ge sp le e1 m1 a t1 e2 m2 (Vint x) ->
-  eval_expr ge sp le e2 m2 b t2 e3 m3 (Vint y) ->
+  forall sp le e m1 a t1 m2 x b t2 m3 y,
+  eval_expr ge sp le e m1 a t1 m2 (Vint x) ->
+  eval_expr ge sp le e m2 b t2 m3 (Vint y) ->
   y <> Int.zero ->
-  eval_expr ge sp le e1 m1 (mods a b) (t1**t2) e3 m3 (Vint (Int.mods x y)).
+  eval_expr ge sp le e m1 (mods a b) (t1**t2) m3 (Vint (Int.mods x y)).
 Proof.
   intros; unfold mods. 
   rewrite Int.mods_divs. 
@@ -740,22 +740,22 @@ Proof.
 Qed.
 
 Lemma eval_divu_base:
-  forall sp le e1 m1 a t1 e2 m2 x b t2 e3 m3 y,
-  eval_expr ge sp le e1 m1 a t1 e2 m2 (Vint x) ->
-  eval_expr ge sp le e2 m2 b t2 e3 m3 (Vint y) ->
+  forall sp le e m1 a t1 m2 x b t2 m3 y,
+  eval_expr ge sp le e m1 a t1 m2 (Vint x) ->
+  eval_expr ge sp le e m2 b t2 m3 (Vint y) ->
   y <> Int.zero ->
-  eval_expr ge sp le e1 m1 (Eop Odivu (a ::: b ::: Enil)) (t1**t2) e3 m3 (Vint (Int.divu x y)).
+  eval_expr ge sp le e m1 (Eop Odivu (a ::: b ::: Enil)) (t1**t2) m3 (Vint (Int.divu x y)).
 Proof.
   intros. EvalOp. simpl. 
   predSpec Int.eq Int.eq_spec y Int.zero. contradiction. auto.
 Qed.
 
 Theorem eval_divu:
-  forall sp le e1 m1 a t1 e2 m2 x b t2 e3 m3 y,
-  eval_expr ge sp le e1 m1 a t1 e2 m2 (Vint x) ->
-  eval_expr ge sp le e2 m2 b t2 e3 m3 (Vint y) ->
+  forall sp le e m1 a t1 m2 x b t2 m3 y,
+  eval_expr ge sp le e m1 a t1 m2 (Vint x) ->
+  eval_expr ge sp le e m2 b t2 m3 (Vint y) ->
   y <> Int.zero ->
-  eval_expr ge sp le e1 m1 (divu a b) (t1**t2) e3 m3 (Vint (Int.divu x y)).
+  eval_expr ge sp le e m1 (divu a b) (t1**t2) m3 (Vint (Int.divu x y)).
 Proof.
   intros until y.
   unfold divu; case (divu_match b); intros.
@@ -768,11 +768,11 @@ Proof.
 Qed.
 
 Theorem eval_modu:
-  forall sp le e1 m1 a t1 e2 m2 x b t2 e3 m3 y,
-  eval_expr ge sp le e1 m1 a t1 e2 m2 (Vint x) ->
-  eval_expr ge sp le e2 m2 b t2 e3 m3 (Vint y) ->
+  forall sp le e m1 a t1 m2 x b t2 m3 y,
+  eval_expr ge sp le e m1 a t1 m2 (Vint x) ->
+  eval_expr ge sp le e m2 b t2 m3 (Vint y) ->
   y <> Int.zero ->
-  eval_expr ge sp le e1 m1 (modu a b) (t1**t2) e3 m3 (Vint (Int.modu x y)).
+  eval_expr ge sp le e m1 (modu a b) (t1**t2) m3 (Vint (Int.modu x y)).
 Proof.
   intros until y; unfold modu; case (divu_match b); intros.
   InvEval H0. caseEq (Int.is_power2 y). 
@@ -789,9 +789,9 @@ Proof.
 Qed.
 
 Theorem eval_andimm:
-  forall sp le e1 m1 n a t e2 m2 x,
-  eval_expr ge sp le e1 m1 a t e2 m2 (Vint x) ->
-  eval_expr ge sp le e1 m1 (andimm n a) t e2 m2 (Vint (Int.and x n)).
+  forall sp le e m1 n a t m2 x,
+  eval_expr ge sp le e m1 a t m2 (Vint x) ->
+  eval_expr ge sp le e m1 (andimm n a) t m2 (Vint (Int.and x n)).
 Proof.
   intros.  unfold andimm. case (Int.is_rlw_mask n).
   rewrite <- Int.rolm_zero. apply eval_rolm; auto.
@@ -799,10 +799,10 @@ Proof.
 Qed.
 
 Theorem eval_and:
-  forall sp le e1 m1 a t1 e2 m2 x b t2 e3 m3 y,
-  eval_expr ge sp le e1 m1 a t1 e2 m2 (Vint x) ->
-  eval_expr ge sp le e2 m2 b t2 e3 m3 (Vint y) ->
-  eval_expr ge sp le e1 m1 (and a b) (t1**t2) e3 m3 (Vint (Int.and x y)).
+  forall sp le e m1 a t1 m2 x b t2 m3 y,
+  eval_expr ge sp le e m1 a t1 m2 (Vint x) ->
+  eval_expr ge sp le e m2 b t2 m3 (Vint y) ->
+  eval_expr ge sp le e m1 (and a b) (t1**t2) m3 (Vint (Int.and x y)).
 Proof.
   intros until y; unfold and; case (mul_match a b); intros.
   InvEval H. rewrite Int.and_commut. 
@@ -812,11 +812,11 @@ Proof.
 Qed.
 
 Remark eval_same_expr_pure:
-  forall a1 a2 sp le e1 m1 t1 e2 m2 v1 t2 e3 m3 v2,
+  forall a1 a2 sp le e m1 t1 m2 v1 t2 m3 v2,
   same_expr_pure a1 a2 = true ->
-  eval_expr ge sp le e1 m1 a1 t1 e2 m2 v1 ->
-  eval_expr ge sp le e2 m2 a2 t2 e3 m3 v2 ->
-  t1 = E0 /\ t2 = E0 /\ a2 = a1 /\ v2 = v1 /\ e2 = e1 /\ m2 = m1.
+  eval_expr ge sp le e m1 a1 t1 m2 v1 ->
+  eval_expr ge sp le e m2 a2 t2 m3 v2 ->
+  t1 = E0 /\ t2 = E0 /\ a2 = a1 /\ v2 = v1 /\ m2 = m1.
 Proof.
   intros until v2.
   destruct a1; simpl; try (intros; discriminate). 
@@ -828,18 +828,18 @@ Proof.
 Qed.
 
 Lemma eval_or:
-  forall sp le e1 m1 a t1 e2 m2 x b t2 e3 m3 y,
-  eval_expr ge sp le e1 m1 a t1 e2 m2 (Vint x) ->
-  eval_expr ge sp le e2 m2 b t2 e3 m3 (Vint y) ->
-  eval_expr ge sp le e1 m1 (or a b) (t1**t2) e3 m3 (Vint (Int.or x y)).
+  forall sp le e m1 a t1 m2 x b t2 m3 y,
+  eval_expr ge sp le e m1 a t1 m2 (Vint x) ->
+  eval_expr ge sp le e m2 b t2 m3 (Vint y) ->
+  eval_expr ge sp le e m1 (or a b) (t1**t2) m3 (Vint (Int.or x y)).
 Proof.
   intros until y; unfold or; case (or_match a b); intros.
   generalize (Int.eq_spec amount1 amount2); case (Int.eq amount1 amount2); intro.
   case (Int.is_rlw_mask (Int.or mask1 mask2)).
   caseEq (same_expr_pure t0 t3); intro.
   simpl. InvEval H. FuncInv. InvEval H0. FuncInv. 
-  generalize (eval_same_expr_pure _ _ _ _ _ _ _ _ _ _ _ _ _ _ H2 EV EV0).
-  intros [EQ1 [EQ2 [EQ3 [EQ4 [EQ5 EQ6]]]]]. 
+  generalize (eval_same_expr_pure _ _ _ _ _ _ _ _ _ _ _ _ H2 EV EV0).
+  intros [EQ1 [EQ2 [EQ3 [EQ4 EQ5]]]]. 
   injection EQ4; intro EQ7. subst.
   EvalOp. simpl. rewrite Int.or_rolm. auto.
   simpl. EvalOp. 
@@ -849,18 +849,18 @@ Proof.
 Qed.
 
 Theorem eval_xor:
-  forall sp le e1 m1 a t1 e2 m2 x b t2 e3 m3 y,
-  eval_expr ge sp le e1 m1 a t1 e2 m2 (Vint x) ->
-  eval_expr ge sp le e2 m2 b t2 e3 m3 (Vint y) ->
-  eval_expr ge sp le e1 m1 (xor a b) (t1**t2) e3 m3 (Vint (Int.xor x y)).
+  forall sp le e m1 a t1 m2 x b t2 m3 y,
+  eval_expr ge sp le e m1 a t1 m2 (Vint x) ->
+  eval_expr ge sp le e m2 b t2 m3 (Vint y) ->
+  eval_expr ge sp le e m1 (xor a b) (t1**t2) m3 (Vint (Int.xor x y)).
 Proof. TrivialOp xor. Qed.
 
 Theorem eval_shl:
-  forall sp le e1 m1 a t1 e2 m2 x b t2 e3 m3 y,
-  eval_expr ge sp le e1 m1 a t1 e2 m2 (Vint x) ->
-  eval_expr ge sp le e2 m2 b t2 e3 m3 (Vint y) ->
+  forall sp le e m1 a t1 m2 x b t2 m3 y,
+  eval_expr ge sp le e m1 a t1 m2 (Vint x) ->
+  eval_expr ge sp le e m2 b t2 m3 (Vint y) ->
   Int.ltu y (Int.repr 32) = true ->
-  eval_expr ge sp le e1 m1 (shl a b) (t1**t2) e3 m3 (Vint (Int.shl x y)).
+  eval_expr ge sp le e m1 (shl a b) (t1**t2) m3 (Vint (Int.shl x y)).
 Proof.
   intros until y; unfold shl; case (shift_match b); intros.
   InvEval H0. rewrite E0_right. apply eval_shlimm; auto.
@@ -868,21 +868,21 @@ Proof.
 Qed.
 
 Theorem eval_shr:
-  forall sp le e1 m1 a t1 e2 m2 x b t2 e3 m3 y,
-  eval_expr ge sp le e1 m1 a t1 e2 m2 (Vint x) ->
-  eval_expr ge sp le e2 m2 b t2 e3 m3 (Vint y) ->
+  forall sp le e m1 a t1 m2 x b t2 m3 y,
+  eval_expr ge sp le e m1 a t1 m2 (Vint x) ->
+  eval_expr ge sp le e m2 b t2 m3 (Vint y) ->
   Int.ltu y (Int.repr 32) = true ->
-  eval_expr ge sp le e1 m1 (shr a b) (t1**t2) e3 m3 (Vint (Int.shr x y)).
+  eval_expr ge sp le e m1 (shr a b) (t1**t2) m3 (Vint (Int.shr x y)).
 Proof.
   TrivialOp shr. simpl. rewrite H1. auto.
 Qed.
 
 Theorem eval_shru:
-  forall sp le e1 m1 a t1 e2 m2 x b t2 e3 m3 y,
-  eval_expr ge sp le e1 m1 a t1 e2 m2 (Vint x) ->
-  eval_expr ge sp le e2 m2 b t2 e3 m3 (Vint y) ->
+  forall sp le e m1 a t1 m2 x b t2 m3 y,
+  eval_expr ge sp le e m1 a t1 m2 (Vint x) ->
+  eval_expr ge sp le e m2 b t2 m3 (Vint y) ->
   Int.ltu y (Int.repr 32) = true ->
-  eval_expr ge sp le e1 m1 (shru a b) (t1**t2) e3 m3 (Vint (Int.shru x y)).
+  eval_expr ge sp le e m1 (shru a b) (t1**t2) m3 (Vint (Int.shru x y)).
 Proof.
   intros until y; unfold shru; case (shift_match b); intros.
   InvEval H0. rewrite E0_right; apply eval_shruimm; auto.
@@ -890,10 +890,10 @@ Proof.
 Qed.
 
 Theorem eval_addf:
-  forall sp le e1 m1 a t1 e2 m2 x b t2 e3 m3 y,
-  eval_expr ge sp le e1 m1 a t1 e2 m2 (Vfloat x) ->
-  eval_expr ge sp le e2 m2 b t2 e3 m3 (Vfloat y) ->
-  eval_expr ge sp le e1 m1 (addf a b) (t1**t2) e3 m3 (Vfloat (Float.add x y)).
+  forall sp le e m1 a t1 m2 x b t2 m3 y,
+  eval_expr ge sp le e m1 a t1 m2 (Vfloat x) ->
+  eval_expr ge sp le e m2 b t2 m3 (Vfloat y) ->
+  eval_expr ge sp le e m1 (addf a b) (t1**t2) m3 (Vfloat (Float.add x y)).
 Proof.
   intros until y; unfold addf; case (addf_match a b); intros.
   InvEval H. FuncInv. EvalOp. 
@@ -909,10 +909,10 @@ Proof.
 Qed.
  
 Theorem eval_subf:
-  forall sp le e1 m1 a t1 e2 m2 x b t2 e3 m3 y,
-  eval_expr ge sp le e1 m1 a t1 e2 m2 (Vfloat x) ->
-  eval_expr ge sp le e2 m2 b t2 e3 m3 (Vfloat y) ->
-  eval_expr ge sp le e1 m1 (subf a b) (t1**t2) e3 m3 (Vfloat (Float.sub x y)).
+  forall sp le e m1 a t1 m2 x b t2 m3 y,
+  eval_expr ge sp le e m1 a t1 m2 (Vfloat x) ->
+  eval_expr ge sp le e m2 b t2 m3 (Vfloat y) ->
+  eval_expr ge sp le e m1 (subf a b) (t1**t2) m3 (Vfloat (Float.sub x y)).
 Proof.
   intros until y; unfold subf; case (subf_match a b); intros.
   InvEval H. FuncInv. EvalOp. 
@@ -922,23 +922,23 @@ Proof.
 Qed.
 
 Theorem eval_mulf:
-  forall sp le e1 m1 a t1 e2 m2 x b t2 e3 m3 y,
-  eval_expr ge sp le e1 m1 a t1 e2 m2 (Vfloat x) ->
-  eval_expr ge sp le e2 m2 b t2 e3 m3 (Vfloat y) ->
-  eval_expr ge sp le e1 m1 (mulf a b) (t1**t2) e3 m3 (Vfloat (Float.mul x y)).
+  forall sp le e m1 a t1 m2 x b t2 m3 y,
+  eval_expr ge sp le e m1 a t1 m2 (Vfloat x) ->
+  eval_expr ge sp le e m2 b t2 m3 (Vfloat y) ->
+  eval_expr ge sp le e m1 (mulf a b) (t1**t2) m3 (Vfloat (Float.mul x y)).
 Proof. TrivialOp mulf. Qed.
 
 Theorem eval_divf:
-  forall sp le e1 m1 a t1 e2 m2 x b t2 e3 m3 y,
-  eval_expr ge sp le e1 m1 a t1 e2 m2 (Vfloat x) ->
-  eval_expr ge sp le e2 m2 b t2 e3 m3 (Vfloat y) ->
-  eval_expr ge sp le e1 m1 (divf a b) (t1**t2) e3 m3 (Vfloat (Float.div x y)).
+  forall sp le e m1 a t1 m2 x b t2 m3 y,
+  eval_expr ge sp le e m1 a t1 m2 (Vfloat x) ->
+  eval_expr ge sp le e m2 b t2 m3 (Vfloat y) ->
+  eval_expr ge sp le e m1 (divf a b) (t1**t2) m3 (Vfloat (Float.div x y)).
 Proof. TrivialOp divf. Qed.
 
 Theorem eval_cast8signed:
-  forall sp le e1 m1 a t e2 m2 v,
-  eval_expr ge sp le e1 m1 a t e2 m2 v ->
-  eval_expr ge sp le e1 m1 (cast8signed a) t e2 m2 (Val.cast8signed v).
+  forall sp le e m1 a t m2 v,
+  eval_expr ge sp le e m1 a t m2 v ->
+  eval_expr ge sp le e m1 (cast8signed a) t m2 (Val.cast8signed v).
 Proof. 
   intros until v; unfold cast8signed; case (cast8signed_match a); intros.
   replace (Val.cast8signed v) with v. auto. 
@@ -947,9 +947,9 @@ Proof.
 Qed.
 
 Theorem eval_cast8unsigned:
-  forall sp le e1 m1 a t e2 m2 v,
-  eval_expr ge sp le e1 m1 a t e2 m2 v ->
-  eval_expr ge sp le e1 m1 (cast8unsigned a) t e2 m2 (Val.cast8unsigned v).
+  forall sp le e m1 a t m2 v,
+  eval_expr ge sp le e m1 a t m2 v ->
+  eval_expr ge sp le e m1 (cast8unsigned a) t m2 (Val.cast8unsigned v).
 Proof. 
   intros until v; unfold cast8unsigned; case (cast8unsigned_match a); intros.
   replace (Val.cast8unsigned v) with v. auto. 
@@ -958,9 +958,9 @@ Proof.
 Qed.
 
 Theorem eval_cast16signed:
-  forall sp le e1 m1 a t e2 m2 v,
-  eval_expr ge sp le e1 m1 a t e2 m2 v ->
-  eval_expr ge sp le e1 m1 (cast16signed a) t e2 m2 (Val.cast16signed v).
+  forall sp le e m1 a t m2 v,
+  eval_expr ge sp le e m1 a t m2 v ->
+  eval_expr ge sp le e m1 (cast16signed a) t m2 (Val.cast16signed v).
 Proof. 
   intros until v; unfold cast16signed; case (cast16signed_match a); intros.
   replace (Val.cast16signed v) with v. auto. 
@@ -969,9 +969,9 @@ Proof.
 Qed.
 
 Theorem eval_cast16unsigned:
-  forall sp le e1 m1 a t e2 m2 v,
-  eval_expr ge sp le e1 m1 a t e2 m2 v ->
-  eval_expr ge sp le e1 m1 (cast16unsigned a) t e2 m2 (Val.cast16unsigned v).
+  forall sp le e m1 a t m2 v,
+  eval_expr ge sp le e m1 a t m2 v ->
+  eval_expr ge sp le e m1 (cast16unsigned a) t m2 (Val.cast16unsigned v).
 Proof. 
   intros until v; unfold cast16unsigned; case (cast16unsigned_match a); intros.
   replace (Val.cast16unsigned v) with v. auto. 
@@ -980,9 +980,9 @@ Proof.
 Qed.
 
 Theorem eval_singleoffloat:
-  forall sp le e1 m1 a t e2 m2 v,
-  eval_expr ge sp le e1 m1 a t e2 m2 v ->
-  eval_expr ge sp le e1 m1 (singleoffloat a) t e2 m2 (Val.singleoffloat v).
+  forall sp le e m1 a t m2 v,
+  eval_expr ge sp le e m1 a t m2 v ->
+  eval_expr ge sp le e m1 (singleoffloat a) t m2 (Val.singleoffloat v).
 Proof. 
   intros until v; unfold singleoffloat; case (singleoffloat_match a); intros.
   replace (Val.singleoffloat v) with v. auto. 
@@ -991,42 +991,42 @@ Proof.
 Qed.
 
 Theorem eval_cmp:
-  forall sp le c e1 m1 a t1 e2 m2 x b t2 e3 m3 y,
-  eval_expr ge sp le e1 m1 a t1 e2 m2 (Vint x) ->
-  eval_expr ge sp le e2 m2 b t2 e3 m3 (Vint y) ->
-  eval_expr ge sp le e1 m1 (cmp c a b) (t1**t2) e3 m3 (Val.of_bool (Int.cmp c x y)).
+  forall sp le c e m1 a t1 m2 x b t2 m3 y,
+  eval_expr ge sp le e m1 a t1 m2 (Vint x) ->
+  eval_expr ge sp le e m2 b t2 m3 (Vint y) ->
+  eval_expr ge sp le e m1 (cmp c a b) (t1**t2) m3 (Val.of_bool (Int.cmp c x y)).
 Proof. 
   TrivialOp cmp. 
   simpl. case (Int.cmp c x y); auto.
 Qed.
 
 Theorem eval_cmp_null_r:
-  forall sp le c e1 m1 a t1 e2 m2 p x b t2 e3 m3 v,
-  eval_expr ge sp le e1 m1 a t1 e2 m2 (Vptr p x) ->
-  eval_expr ge sp le e2 m2 b t2 e3 m3 (Vint Int.zero) ->
+  forall sp le c e m1 a t1 m2 p x b t2 m3 v,
+  eval_expr ge sp le e m1 a t1 m2 (Vptr p x) ->
+  eval_expr ge sp le e m2 b t2 m3 (Vint Int.zero) ->
   (c = Ceq /\ v = Vfalse) \/ (c = Cne /\ v = Vtrue) ->
-  eval_expr ge sp le e1 m1 (cmp c a b) (t1**t2) e3 m3 v.
+  eval_expr ge sp le e m1 (cmp c a b) (t1**t2) m3 v.
 Proof. 
   TrivialOp cmp. 
   simpl. elim H1; intros [EQ1 EQ2]; subst c; subst v; reflexivity.
 Qed.
 
 Theorem eval_cmp_null_l:
-  forall sp le c e1 m1 a t1 e2 m2 p x b t2 e3 m3 v,
-  eval_expr ge sp le e1 m1 a t1 e2 m2 (Vint Int.zero) ->
-  eval_expr ge sp le e2 m2 b t2 e3 m3 (Vptr p x) ->
+  forall sp le c e m1 a t1 m2 p x b t2 m3 v,
+  eval_expr ge sp le e m1 a t1 m2 (Vint Int.zero) ->
+  eval_expr ge sp le e m2 b t2 m3 (Vptr p x) ->
   (c = Ceq /\ v = Vfalse) \/ (c = Cne /\ v = Vtrue) ->
-  eval_expr ge sp le e1 m1 (cmp c a b) (t1**t2) e3 m3 v.
+  eval_expr ge sp le e m1 (cmp c a b) (t1**t2) m3 v.
 Proof. 
   TrivialOp cmp. 
   simpl. elim H1; intros [EQ1 EQ2]; subst c; subst v; reflexivity.
 Qed.
 
 Theorem eval_cmp_ptr:
-  forall sp le c e1 m1 a t1 e2 m2 p x b t2 e3 m3 y,
-  eval_expr ge sp le e1 m1 a t1 e2 m2 (Vptr p x) ->
-  eval_expr ge sp le e2 m2 b t2 e3 m3 (Vptr p y) ->
-  eval_expr ge sp le e1 m1 (cmp c a b) (t1**t2) e3 m3 (Val.of_bool (Int.cmp c x y)).
+  forall sp le c e m1 a t1 m2 p x b t2 m3 y,
+  eval_expr ge sp le e m1 a t1 m2 (Vptr p x) ->
+  eval_expr ge sp le e m2 b t2 m3 (Vptr p y) ->
+  eval_expr ge sp le e m1 (cmp c a b) (t1**t2) m3 (Val.of_bool (Int.cmp c x y)).
 Proof. 
   TrivialOp cmp. 
   simpl. unfold eq_block. rewrite zeq_true. 
@@ -1034,32 +1034,32 @@ Proof.
 Qed.
 
 Theorem eval_cmpu:
-  forall sp le c e1 m1 a t1 e2 m2 x b t2 e3 m3 y,
-  eval_expr ge sp le e1 m1 a t1 e2 m2 (Vint x) ->
-  eval_expr ge sp le e2 m2 b t2 e3 m3 (Vint y) ->
-  eval_expr ge sp le e1 m1 (cmpu c a b) (t1**t2) e3 m3 (Val.of_bool (Int.cmpu c x y)).
+  forall sp le c e m1 a t1 m2 x b t2 m3 y,
+  eval_expr ge sp le e m1 a t1 m2 (Vint x) ->
+  eval_expr ge sp le e m2 b t2 m3 (Vint y) ->
+  eval_expr ge sp le e m1 (cmpu c a b) (t1**t2) m3 (Val.of_bool (Int.cmpu c x y)).
 Proof. 
   TrivialOp cmpu. 
   simpl. case (Int.cmpu c x y); auto.
 Qed.
 
 Theorem eval_cmpf:
-  forall sp le c e1 m1 a t1 e2 m2 x b t2 e3 m3 y,
-  eval_expr ge sp le e1 m1 a t1 e2 m2 (Vfloat x) ->
-  eval_expr ge sp le e2 m2 b t2 e3 m3 (Vfloat y) ->
-  eval_expr ge sp le e1 m1 (cmpf c a b) (t1**t2) e3 m3 (Val.of_bool (Float.cmp c x y)).
+  forall sp le c e m1 a t1 m2 x b t2 m3 y,
+  eval_expr ge sp le e m1 a t1 m2 (Vfloat x) ->
+  eval_expr ge sp le e m2 b t2 m3 (Vfloat y) ->
+  eval_expr ge sp le e m1 (cmpf c a b) (t1**t2) m3 (Val.of_bool (Float.cmp c x y)).
 Proof. 
   TrivialOp cmpf. 
   simpl. case (Float.cmp c x y); auto.
 Qed.
 
 Lemma eval_base_condition_of_expr:
-  forall sp le a e1 m1 t e2 m2 v (b: bool),
-  eval_expr ge sp le e1 m1 a t e2 m2 v ->
+  forall sp le a e m1 t m2 v (b: bool),
+  eval_expr ge sp le e m1 a t m2 v ->
   Val.bool_of_val v b ->
-  eval_condexpr ge sp le e1 m1 
+  eval_condexpr ge sp le e m1 
                 (CEcond (Ccompuimm Cne Int.zero) (a ::: Enil))
-                t e2 m2 b.
+                t m2 b.
 Proof.
   intros. 
   eapply eval_CEcond. eauto with evalexpr. 
@@ -1067,60 +1067,60 @@ Proof.
 Qed.
 
 Lemma eval_condition_of_expr:
-  forall a sp le e1 m1 t e2 m2 v (b: bool),
-  eval_expr ge sp le e1 m1 a t e2 m2 v ->
+  forall a sp le e m1 t m2 v (b: bool),
+  eval_expr ge sp le e m1 a t m2 v ->
   Val.bool_of_val v b ->
-  eval_condexpr ge sp le e1 m1 (condexpr_of_expr a) t e2 m2 b.
+  eval_condexpr ge sp le e m1 (condexpr_of_expr a) t m2 b.
 Proof.
   induction a; simpl; intros;
     try (eapply eval_base_condition_of_expr; eauto; fail).
   destruct o; try (eapply eval_base_condition_of_expr; eauto; fail).
 
-  destruct e. InvEval H. inversion XX4; subst v.
+  destruct e. InvEval H. inversion XX3; subst v.
   inversion H0. 
   rewrite Int.eq_false; auto. constructor.
   subst i; rewrite Int.eq_true. constructor.
   eapply eval_base_condition_of_expr; eauto.
 
-  inversion H. subst. eapply eval_CEcond; eauto. simpl in H12.
+  inversion H. subst. eapply eval_CEcond; eauto. simpl in H11.
   destruct (eval_condition c vl); try discriminate.
-  destruct b0; inversion H12; subst; inversion H0; congruence.
+  destruct b0; inversion H11; subst; inversion H0; congruence.
 
   inversion H. subst.
   destruct v1; eauto with evalexpr.
 Qed.
 
 Theorem eval_conditionalexpr_true:
-  forall sp le e1 m1 a1 t1 e2 m2 v1 t2 a2 e3 m3 v2 a3,
-  eval_expr ge sp le e1 m1 a1 t1 e2 m2 v1 ->
+  forall sp le e m1 a1 t1 m2 v1 t2 a2 m3 v2 a3,
+  eval_expr ge sp le e m1 a1 t1 m2 v1 ->
   Val.is_true v1 ->
-  eval_expr ge sp le e2 m2 a2 t2 e3 m3 v2 ->
-  eval_expr ge sp le e1 m1 (conditionalexpr a1 a2 a3) (t1**t2) e3 m3 v2.
+  eval_expr ge sp le e m2 a2 t2 m3 v2 ->
+  eval_expr ge sp le e m1 (conditionalexpr a1 a2 a3) (t1**t2) m3 v2.
 Proof.
   intros; unfold conditionalexpr.
-  apply eval_Econdition with t1 e2 m2 true t2; auto.
+  apply eval_Econdition with t1 m2 true t2; auto.
   eapply eval_condition_of_expr; eauto with valboolof.
 Qed.
 
 Theorem eval_conditionalexpr_false:
-  forall sp le e1 m1 a1 t1 e2 m2 v1 a2 t2 e3 m3 v2 a3,
-  eval_expr ge sp le e1 m1 a1 t1 e2 m2 v1 ->
+  forall sp le e m1 a1 t1 m2 v1 a2 t2 m3 v2 a3,
+  eval_expr ge sp le e m1 a1 t1 m2 v1 ->
   Val.is_false v1 ->
-  eval_expr ge sp le e2 m2 a3 t2 e3 m3 v2 ->
-  eval_expr ge sp le e1 m1 (conditionalexpr a1 a2 a3) (t1**t2) e3 m3 v2.
+  eval_expr ge sp le e m2 a3 t2 m3 v2 ->
+  eval_expr ge sp le e m1 (conditionalexpr a1 a2 a3) (t1**t2) m3 v2.
 Proof.
   intros; unfold conditionalexpr.
-  apply eval_Econdition with t1 e2 m2 false t2; auto.
+  apply eval_Econdition with t1 m2 false t2; auto.
   eapply eval_condition_of_expr; eauto with valboolof.
 Qed.
 
 Lemma eval_addressing:
-  forall sp le e1 m1 a t e2 m2 v b ofs,
-  eval_expr ge sp le e1 m1 a t e2 m2 v ->
+  forall sp le e m1 a t m2 v b ofs,
+  eval_expr ge sp le e m1 a t m2 v ->
   v = Vptr b ofs ->
   match addressing a with (mode, args) =>
     exists vl,
-    eval_exprlist ge sp le e1 m1 args t e2 m2 vl /\ 
+    eval_exprlist ge sp le e m1 args t m2 vl /\ 
     eval_addressing ge sp mode vl = Some v
   end.
 Proof.
@@ -1151,54 +1151,54 @@ Proof.
 Qed.
 
 Theorem eval_load:
-  forall sp le e1 m1 a t e2 m2 v chunk v',
-  eval_expr ge sp le e1 m1 a t e2 m2 v ->
+  forall sp le e m1 a t m2 v chunk v',
+  eval_expr ge sp le e m1 a t m2 v ->
   Mem.loadv chunk m2 v = Some v' ->
-  eval_expr ge sp le e1 m1 (load chunk a) t e2 m2 v'.
+  eval_expr ge sp le e m1 (load chunk a) t m2 v'.
 Proof.
   intros. generalize H0; destruct v; simpl; intro; try discriminate.
   unfold load. 
-  generalize (eval_addressing _ _ _ _ _ _ _ _ _ _ _ H (refl_equal _)).
+  generalize (eval_addressing _ _ _ _ _ _ _ _ _ _ H (refl_equal _)).
   destruct (addressing a). intros [vl [EV EQ]]. 
   eapply eval_Eload; eauto. 
 Qed.
 
 Theorem eval_store:
-  forall sp le e1 m1 a1 t1 e2 m2 v1 a2 t2 e3 m3 v2 chunk m4,
-  eval_expr ge sp le e1 m1 a1 t1 e2 m2 v1 ->
-  eval_expr ge sp le e2 m2 a2 t2 e3 m3 v2 ->
+  forall sp le e m1 a1 t1 m2 v1 a2 t2 m3 v2 chunk m4,
+  eval_expr ge sp le e m1 a1 t1 m2 v1 ->
+  eval_expr ge sp le e m2 a2 t2 m3 v2 ->
   Mem.storev chunk m3 v1 v2 = Some m4 ->
-  eval_expr ge sp le e1 m1 (store chunk a1 a2) (t1**t2) e3 m4 v2.
+  eval_expr ge sp le e m1 (store chunk a1 a2) (t1**t2) m4 v2.
 Proof.
   intros. generalize H1; destruct v1; simpl; intro; try discriminate.
   unfold store.
-  generalize (eval_addressing _ _ _ _ _ _ _ _ _ _ _ H (refl_equal _)).
+  generalize (eval_addressing _ _ _ _ _ _ _ _ _ _ H (refl_equal _)).
   destruct (addressing a1). intros [vl [EV EQ]]. 
   eapply eval_Estore; eauto. 
 Qed.
 
 Theorem exec_ifthenelse_true:
-  forall sp e1 m1 a t1 e2 m2 v ifso ifnot t2 e3 m3 out,
-  eval_expr ge sp nil e1 m1 a t1 e2 m2 v ->
+  forall sp e m1 a t1 m2 v ifso ifnot t2 e3 m3 out,
+  eval_expr ge sp nil e m1 a t1 m2 v ->
   Val.is_true v ->
-  exec_stmt ge sp e2 m2 ifso t2 e3 m3 out ->
-  exec_stmt ge sp e1 m1 (ifthenelse a ifso ifnot) (t1**t2) e3 m3 out.
+  exec_stmt ge sp e m2 ifso t2 e3 m3 out ->
+  exec_stmt ge sp e m1 (ifthenelse a ifso ifnot) (t1**t2) e3 m3 out.
 Proof.
   intros. unfold ifthenelse.
-  apply exec_Sifthenelse with t1 e2 m2 true t2.
+  apply exec_Sifthenelse with t1 m2 true t2.
   eapply eval_condition_of_expr; eauto with valboolof.
   auto. auto.
 Qed.
 
 Theorem exec_ifthenelse_false:
-  forall sp e1 m1 a t1 e2 m2 v ifso ifnot t2 e3 m3 out,
-  eval_expr ge sp nil e1 m1 a t1 e2 m2 v ->
+  forall sp e m1 a t1 m2 v ifso ifnot t2 e3 m3 out,
+  eval_expr ge sp nil e m1 a t1 m2 v ->
   Val.is_false v ->
-  exec_stmt ge sp e2 m2 ifnot t2 e3 m3 out ->
-  exec_stmt ge sp e1 m1 (ifthenelse a ifso ifnot) (t1**t2) e3 m3 out.
+  exec_stmt ge sp e m2 ifnot t2 e3 m3 out ->
+  exec_stmt ge sp e m1 (ifthenelse a ifso ifnot) (t1**t2) e3 m3 out.
 Proof.
   intros. unfold ifthenelse.
-  apply exec_Sifthenelse with t1 e2 m2 false t2.
+  apply exec_Sifthenelse with t1 m2 false t2.
   eapply eval_condition_of_expr; eauto with valboolof.
   auto. auto.
 Qed.
